James C - cleaning up the mess in debranching

Debranching.thy
@@ -31,14 +31,14 @@ primrec block_convert :: "code_label set \<Rightarrow> code_label \<times> b_ass
 definition debranch :: "b_assembly_program \<Rightarrow> assembly_program" where
   "debranch \<Pi> = finite_map_fold (block_convert (dom \<Pi>)) empty \<Pi>"
 
-function code_join :: "assembly list \<Rightarrow> assembly_program \<Rightarrow> assembly list set" where
-  "code_join \<pi> \<Pi> = (
+function jump_join :: "assembly list \<Rightarrow> assembly_program \<Rightarrow> assembly list set" where
+  "jump_join \<pi> \<Pi> = (
     if finite (dom \<Pi>)
     then case last \<pi> of
         JAssm jmp s \<Rightarrow> (
           if jmp = {GT, EQ, LT} 
           then case \<Pi> s of 
-              Some \<pi>' \<Rightarrow> insert \<pi> (code_join (butlast \<pi> @ \<pi>') (\<Pi>(s := None)))
+              Some \<pi>' \<Rightarrow> insert \<pi> (jump_join (butlast \<pi> @ \<pi>') (\<Pi>(s := None)))
             | None \<Rightarrow> {\<pi>} 
           else {\<pi>})
       | _ \<Rightarrow> {\<pi>}
@@ -50,7 +50,7 @@ termination
 fun state_convert :: "code_label set \<Rightarrow> b_assembly_state \<Rightarrow> assembly_state set" where
   "state_convert ss (\<mu>, a, d, \<pi>, \<omega>) = (
     let (\<pi>', \<Pi>) = branch_instr_convert ss \<pi> 
-    in {(\<mu>, a, d, \<pi>'', \<omega>) | \<pi>''. \<pi>'' \<in> code_join \<pi>' \<Pi>})"
+    in {(\<mu>, a, d, \<pi>'', \<omega>) | \<pi>''. \<pi>'' \<in> jump_join \<pi>' \<Pi>})"
 
 (* conversion correctness *)
 
@@ -109,65 +109,50 @@ lemma [simp]: "finite ss \<Longrightarrow> ss \<supseteq> dom \<Pi> \<Longrighta
 lemma [simp]: "finite (dom \<Pi>) \<Longrightarrow> finite (dom (debranch \<Pi>))"
   by (simp add: debranch_def)
 
-lemma [simp]: "\<pi> \<in> code_join \<pi> \<Pi>"
+lemma [simp]: "\<pi> \<in> jump_join \<pi> \<Pi>"
   by (cases "last \<pi>") (simp_all split: option.splits)
+
+lemma jump_join_a: "\<pi>' \<in> jump_join (AAssm x # \<pi>) \<Pi> \<Longrightarrow> 
+    \<exists>\<pi>''. \<pi>' = AAssm x # \<pi>'' \<and> \<pi>'' \<in> jump_join \<pi> \<Pi>"
+  proof (induction "AAssm x # \<pi>" \<Pi> rule: jump_join.induct)
+  case (1 \<Pi>)
+    thus ?case
+      proof (cases "finite (dom \<Pi>)")
+      case True
+        from 1 True have "
+            last (AAssm x # \<pi>) = JAssm jmp s \<Longrightarrow>
+            jmp = {GT, EQ, LT} \<Longrightarrow>
+            \<Pi> s = Some pi \<Longrightarrow>
+            butlast (AAssm x # \<pi>) @ pi = AAssm x # \<pi> \<Longrightarrow> \<pi>' \<in> jump_join (AAssm x # \<pi>) (\<Pi>(s := None)) \<Longrightarrow> \<exists>\<pi>''. \<pi>' = AAssm x # \<pi>'' \<and> \<pi>'' \<in> jump_join \<pi> (\<Pi>(s := None))" by simp
+        from 1 True have "\<pi>' \<in> (
+        case last (AAssm x # \<pi>) of
+            JAssm jmp s \<Rightarrow> (
+              if jmp = {GT, EQ, LT} 
+              then case \<Pi> s of 
+                  Some \<pi>' \<Rightarrow> insert (AAssm x # \<pi>) (jump_join (butlast (AAssm x # \<pi>) @ \<pi>') (\<Pi>(s := None)))
+                | None \<Rightarrow> {AAssm x # \<pi>} 
+              else {AAssm x # \<pi>})
+          | _ \<Rightarrow> {AAssm x # \<pi>})" by simp
+    
+    
+        have "\<pi>' = AAssm x # \<pi>'' \<and> \<pi>'' \<in> (
+        case last \<pi> of
+            JAssm jmp s \<Rightarrow> (
+              if jmp = {GT, EQ, LT} 
+              then case \<Pi> s of 
+                  Some \<pi>' \<Rightarrow> insert \<pi> (jump_join (butlast \<pi> @ \<pi>') (\<Pi>(s := None)))
+                | None \<Rightarrow> {\<pi>} 
+              else {\<pi>})
+          | _ \<Rightarrow> {\<pi>})" by simp
+        with True show ?thesis by simp
+      next case False
+        with 1 show ?thesis by simp
+      qed
+  qed
 
 lemma [simp]: "\<Sigma>\<^sub>A \<in> state_convert ss \<Sigma>\<^sub>B \<Longrightarrow> assembly_output \<Sigma>\<^sub>A = b_assembly_output \<Sigma>\<^sub>B"
   by (induction \<Sigma>\<^sub>B rule: b_assembly_output.induct, induction \<Sigma>\<^sub>A rule: assembly_output.induct) 
      (simp split: prod.splits)
-
-lemma [simp]: "branch_instr_convert (dom \<Pi>) \<pi>\<^sub>B = (\<pi>\<^sub>A, \<Pi>') \<Longrightarrow> 
-    (\<mu>, a, d, \<pi>\<^sub>A, \<omega>) \<in> state_convert (dom \<Pi>) (\<mu>, a, d, \<pi>\<^sub>B, \<omega>)" 
-  by simp
-
-lemma [simp]: "finite ss \<Longrightarrow> ss \<supseteq> dom \<Pi> \<Longrightarrow> \<Pi> s = Some \<pi>\<^sub>B \<Longrightarrow> 
-    branch_instr_convert ss \<pi>\<^sub>B = (\<pi>\<^sub>A, \<Pi>') \<Longrightarrow> finite_map_fold (block_convert ss) empty \<Pi> s = Some \<pi>\<^sub>A"
-  proof (induction "block_convert ss" "empty :: code_label \<Rightarrow> assembly list option" \<Pi> 
-         rule: finite_map_fold.induct)
-  case 1
-    thus ?case by (metis finite_subset)
-  next case 2
-    thus ?case by (metis card_0_eq dom_eq_empty_conv option.distinct(1))
-  next case (3 \<Pi>)
-    let ?x = "SOME x. x \<in> dom \<Pi>"
-    let ?ih = "finite_map_fold (block_convert ss) empty (\<Pi>(?x := None))"
-    show ?case 
-      proof (cases "?x = s")
-      case True
-        from 3 have "finite (dom \<Pi>)" by simp
-        from 3 have "card (dom \<Pi>) \<noteq> 0" by simp
-        from 3 have "(\<Pi>(?x := None)) s = Some \<pi>\<^sub>B \<Longrightarrow> ?ih s = Some \<pi>\<^sub>A" by auto
-        from 3 have "finite ss" by simp
-        from 3 have "dom \<Pi> \<subseteq> ss" by simp
-        from 3 have "\<Pi> s = Some \<pi>\<^sub>B" by simp
-        from 3 have "branch_instr_convert ss \<pi>\<^sub>B = (\<pi>\<^sub>A, \<Pi>')" by simp
-    
-    
-
-        have "(let (\<pi>', \<Pi>') = branch_instr_convert (ss \<union> dom ?ih) \<pi>\<^sub>B in \<Pi>'(s \<mapsto> \<pi>')) s = Some \<pi>\<^sub>A" by simp
-        with 3 have "(let (\<pi>', \<Pi>') = 
-          branch_instr_convert (ss \<union> dom ?ih) (the (\<Pi> s)) in \<Pi>'(s \<mapsto> \<pi>')) s = Some \<pi>\<^sub>A" by simp
-        with True have "block_convert ss (?x, the (\<Pi> ?x)) ?ih s = Some \<pi>\<^sub>A" by simp
-        with 3 show ?thesis by (simp add: Let_def)  
-      next case False
-        from 3 have "finite (dom \<Pi>)" by simp
-        from 3 have "card (dom \<Pi>) \<noteq> 0" by simp
-        from 3 have "(\<Pi>(?x := None)) s = Some \<pi>\<^sub>B \<Longrightarrow> ?ih s = Some \<pi>\<^sub>A" by auto
-        from 3 have "finite ss" by simp
-        from 3 have "dom \<Pi> \<subseteq> ss" by simp
-        from 3 have "\<Pi> s = Some \<pi>\<^sub>B" by simp
-        from 3 have "branch_instr_convert ss \<pi>\<^sub>B = (\<pi>\<^sub>A, \<Pi>')" by simp
-    
-
-    
-        have "(let (\<pi>', \<Pi>') = branch_instr_convert (ss \<union> dom ?ih) (the (\<Pi> ?x)) in \<Pi>'(?x \<mapsto> \<pi>')) s = Some \<pi>\<^sub>A" by simp
-        with 3 show ?thesis by (simp add: Let_def)  
-      qed
-  qed
-
-lemma [simp]: "finite (dom \<Pi>) \<Longrightarrow> \<Pi> s = Some \<pi>\<^sub>B \<Longrightarrow> branch_instr_convert (dom \<Pi>) \<pi>\<^sub>B = (\<pi>\<^sub>A, \<Pi>') \<Longrightarrow> 
-    debranch \<Pi> s = Some \<pi>\<^sub>A"
-  by (simp add: debranch_def)
 
 lemma debranch_step: "eval_b_assembly \<Pi> \<Sigma>\<^sub>B = Some \<Sigma>\<^sub>B' \<Longrightarrow> finite (dom \<Pi>) \<Longrightarrow> 
   \<Sigma>\<^sub>A \<in> state_convert (dom \<Pi>) \<Sigma>\<^sub>B \<Longrightarrow> 
@@ -178,78 +163,26 @@ lemma debranch_step: "eval_b_assembly \<Pi> \<Sigma>\<^sub>B = Some \<Sigma>\<^s
   next case (2 \<Pi> \<mu> a d x \<pi> \<omega>)
     thus ?case
       proof (cases "branch_instr_convert (dom \<Pi>) \<pi>")
-      case (Pair \<pi>' \<Pi>')
-        hence S: "(\<mu>, a, d, AAssm x # \<pi>', \<omega>) \<in> state_convert (dom \<Pi>) (\<mu>, a, d, ABAssm x # \<pi>, \<omega>)" 
+      case (Pair \<pi>\<^sub>A \<Pi>\<^sub>A)
+        with 2 obtain \<pi>\<^sub>A' where P: "\<Sigma>\<^sub>A = (\<mu>, a, d, \<pi>\<^sub>A', \<omega>) \<and> \<pi>\<^sub>A' \<in> jump_join (AAssm x # \<pi>\<^sub>A) \<Pi>\<^sub>A" 
+          by auto
+        then obtain \<pi>\<^sub>A'' where P': "\<pi>\<^sub>A' = AAssm x # \<pi>\<^sub>A'' \<and> \<pi>\<^sub>A'' \<in> jump_join \<pi>\<^sub>A \<Pi>\<^sub>A" 
+          by (metis jump_join_a)
+        from 2 have S: "\<Sigma>\<^sub>B' = (\<mu>, Some x, d, \<pi>, \<omega>)" by simp
+        from P' Pair have "(\<mu>, Some x, d, \<pi>\<^sub>A'', \<omega>) \<in> state_convert (dom \<Pi>) (\<mu>, Some x, d, \<pi>, \<omega>)" 
           by simp
-        from Pair have "(\<mu>, Some x, d, \<pi>', \<omega>) \<in> state_convert (dom \<Pi>) (\<mu>, Some x, d, \<pi>, \<omega>)" by simp
-        with 2 S show ?thesis by (simp add: iter_one)
+        with S P P' iter_one eval_assembly.simps(2) show ?thesis by metis
       qed
   next case (3 \<Pi> \<mu> a d dst cmp \<pi> \<omega>)
-    let ?n = "compute cmp (\<mu> a) a d"
-    let ?\<mu> = "if M \<in> dst then \<mu>(a := ?n) else \<mu>"
-    let ?a = "Some (if A \<in> dst then ?n else a)"
-    let ?d = "if D \<in> dst then ?n else d"
-    show ?case
-      proof (cases "branch_instr_convert (dom \<Pi>) \<pi>")
-      case (Pair \<pi>' \<Pi>')
-        hence S: "(?\<mu>, ?a, ?d, \<pi>', \<omega>) \<in> state_convert (dom \<Pi>) (?\<mu>, ?a, ?d, \<pi>, \<omega>)" by simp
-        from Pair have S': "(\<mu>, Some a, d, CAssm dst cmp # \<pi>', \<omega>) \<in> 
-          state_convert (dom \<Pi>) (\<mu>, Some a, d, CBAssm dst cmp # \<pi>, \<omega>)" by simp
-        have "iterate (eval_assembly (debranch \<Pi>)) (\<mu>, Some a, d, CAssm dst cmp # \<pi>', \<omega>) 
-          (?\<mu>, ?a, ?d, \<pi>', \<omega>)" by (meson iter_one eval_assembly.simps(3))
-        with 3 S S' show ?thesis by (simp add: Let_def)
-      qed
+    thus ?case by simp
   next case 4
     thus ?case by simp
   next case (5 \<Pi> \<mu> a d jmp \<pi>\<^sub>t \<pi>\<^sub>f \<pi> \<omega>)
-    show ?case
-      proof (cases "branch_instr_convert (dom \<Pi>) \<pi>\<^sub>t")
-      case (Pair \<pi>\<^sub>t' \<Pi>\<^sub>1) note PT = Pair
-        thus ?thesis
-          proof (cases "branch_instr_convert (dom \<Pi> \<union> dom \<Pi>\<^sub>1) \<pi>\<^sub>f")
-          case (Pair \<pi>\<^sub>f' \<Pi>\<^sub>2) note PF = Pair
-            thus ?thesis 
-              proof (cases "branch_instr_convert (dom \<Pi> \<union> dom \<Pi>\<^sub>1 \<union> dom \<Pi>\<^sub>2) \<pi>")
-              case (Pair \<pi>' \<Pi>\<^sub>3)
-                let ?s\<^sub>t = "new_label (dom \<Pi> \<union> dom \<Pi>\<^sub>1 \<union> dom \<Pi>\<^sub>2 \<union> dom \<Pi>\<^sub>3)"
-                let ?s\<^sub>e = "new_label (dom \<Pi> \<union> dom \<Pi>\<^sub>1 \<union> dom \<Pi>\<^sub>2 \<union> dom \<Pi>\<^sub>3 \<union> {?s\<^sub>t})"
-
-                from 5 have "finite (dom \<Pi>)" by simp
-                                
-                have "state_convert (dom \<Pi>) (\<mu>, a, d, IBAssm jmp \<pi>\<^sub>t \<pi>\<^sub>f # \<pi>, \<omega>) = xxx" by simp
-                
-            
-                have "iterate (eval_assembly (debranch \<Pi>)) (\<mu>, a, d, JAssm jmp ?s\<^sub>t # \<pi>\<^sub>f' @ [JAssm {EQ, LT, GT} ?s\<^sub>e], \<omega>) (state_convert (dom \<Pi>) (\<mu>, a, d, (if should_jump d jmp then \<pi>\<^sub>t else \<pi>\<^sub>f) @ \<pi>, \<omega>))" by simp
-                with PT PF Pair 5 show ?thesis by (simp add: Let_def)
-              qed
-          qed
-      qed
+    thus ?case by simp
   next case (6 \<Pi> \<mu> a d s \<pi> \<omega>)
-    thus ?case
-      proof (cases "\<Pi> s")
-      case (Some \<pi>\<^sub>2)
-        thus ?thesis
-          proof (cases "branch_instr_convert (dom \<Pi>) \<pi>\<^sub>2")
-          case (Pair \<pi>\<^sub>2' \<Pi>')
-            hence S: "(\<mu>, None, d, \<pi>\<^sub>2', \<omega>) \<in> state_convert (dom \<Pi>) (\<mu>, None, d, \<pi>\<^sub>2, \<omega>)" by simp
-            from Some Pair 6 have "eval_assembly (debranch \<Pi>) (\<mu>, a, d, [JAssm {EQ, LT, GT} s], \<omega>) = 
-              Some (\<mu>, None, d, \<pi>\<^sub>2', \<omega>)" by auto
-            hence "iterate (eval_assembly (debranch \<Pi>)) (\<mu>, a, d, [JAssm {EQ, LT, GT} s], \<omega>) 
-              (\<mu>, None, d, \<pi>\<^sub>2', \<omega>)" by (metis iter_one)
-            with 6 Some S show ?thesis by simp
-          qed
-      next case None
-        with 6 show ?thesis by simp
-      qed
+    thus ?case by simp
   next case (7 \<Pi> \<mu> a d \<pi> \<omega>)
-    thus ?case
-      proof (cases "branch_instr_convert (dom \<Pi>) \<pi>")
-      case (Pair \<pi>' \<Pi>')
-        hence S: "(\<mu>, a, d, PAssm # \<pi>', \<omega>) \<in> state_convert (dom \<Pi>) (\<mu>, a, d, PBAssm # \<pi>, \<omega>)" 
-          by simp
-        from Pair have "(\<mu>, a, d, \<pi>', d # \<omega>) \<in> state_convert (dom \<Pi>) (\<mu>, a, d, \<pi>, d # \<omega>)" by simp
-        with 7 S show ?thesis by (simp add: iter_one)
-      qed
+    thus ?case by simp
   qed 
 
 theorem debranching_correct [simp]: "iterate (eval_b_assembly \<Pi>) \<Sigma>\<^sub>B \<Sigma>\<^sub>B' \<Longrightarrow> finite (dom \<Pi>) \<Longrightarrow>
